Add generated Revm primitive spec id types

RocqOfRust/revm/types.v
@@ -8381,3 +8381,359 @@ Module PrecompileSpecId.
 
   End SubPointer.
 End PrecompileSpecId.
+
+Module SpecId.
+  Inductive t : Set :=
+  | FRONTIER
+  | FRONTIER_THAWING
+  | HOMESTEAD
+  | DAO_FORK
+  | TANGERINE
+  | SPURIOUS_DRAGON
+  | BYZANTIUM
+  | CONSTANTINOPLE
+  | PETERSBURG
+  | ISTANBUL
+  | MUIR_GLACIER
+  | BERLIN
+  | LONDON
+  | ARROW_GLACIER
+  | GRAY_GLACIER
+  | MERGE
+  | SHANGHAI
+  | CANCUN
+  | PRAGUE
+  | OSAKA
+  | AMSTERDAM
+  .
+
+  Global Instance IsLink : Link t := {
+    Φ := Ty.path "revm_primitives::hardfork::SpecId";
+    φ x :=
+      match x with
+      | FRONTIER =>
+        Value.StructTuple "revm_primitives::hardfork::SpecId::FRONTIER" []
+      | FRONTIER_THAWING =>
+        Value.StructTuple "revm_primitives::hardfork::SpecId::FRONTIER_THAWING" []
+      | HOMESTEAD =>
+        Value.StructTuple "revm_primitives::hardfork::SpecId::HOMESTEAD" []
+      | DAO_FORK =>
+        Value.StructTuple "revm_primitives::hardfork::SpecId::DAO_FORK" []
+      | TANGERINE =>
+        Value.StructTuple "revm_primitives::hardfork::SpecId::TANGERINE" []
+      | SPURIOUS_DRAGON =>
+        Value.StructTuple "revm_primitives::hardfork::SpecId::SPURIOUS_DRAGON" []
+      | BYZANTIUM =>
+        Value.StructTuple "revm_primitives::hardfork::SpecId::BYZANTIUM" []
+      | CONSTANTINOPLE =>
+        Value.StructTuple "revm_primitives::hardfork::SpecId::CONSTANTINOPLE" []
+      | PETERSBURG =>
+        Value.StructTuple "revm_primitives::hardfork::SpecId::PETERSBURG" []
+      | ISTANBUL =>
+        Value.StructTuple "revm_primitives::hardfork::SpecId::ISTANBUL" []
+      | MUIR_GLACIER =>
+        Value.StructTuple "revm_primitives::hardfork::SpecId::MUIR_GLACIER" []
+      | BERLIN =>
+        Value.StructTuple "revm_primitives::hardfork::SpecId::BERLIN" []
+      | LONDON =>
+        Value.StructTuple "revm_primitives::hardfork::SpecId::LONDON" []
+      | ARROW_GLACIER =>
+        Value.StructTuple "revm_primitives::hardfork::SpecId::ARROW_GLACIER" []
+      | GRAY_GLACIER =>
+        Value.StructTuple "revm_primitives::hardfork::SpecId::GRAY_GLACIER" []
+      | MERGE =>
+        Value.StructTuple "revm_primitives::hardfork::SpecId::MERGE" []
+      | SHANGHAI =>
+        Value.StructTuple "revm_primitives::hardfork::SpecId::SHANGHAI" []
+      | CANCUN =>
+        Value.StructTuple "revm_primitives::hardfork::SpecId::CANCUN" []
+      | PRAGUE =>
+        Value.StructTuple "revm_primitives::hardfork::SpecId::PRAGUE" []
+      | OSAKA =>
+        Value.StructTuple "revm_primitives::hardfork::SpecId::OSAKA" []
+      | AMSTERDAM =>
+        Value.StructTuple "revm_primitives::hardfork::SpecId::AMSTERDAM" []
+      end
+  }.
+
+  Definition of_ty : OfTy.t (Ty.path "revm_primitives::hardfork::SpecId").
+  Proof. eapply OfTy.Make with (A := t); reflexivity. Defined.
+  Smpl Add simple apply of_ty : of_ty.
+
+  Lemma of_value_with_FRONTIER :
+    Value.StructTuple "revm_primitives::hardfork::SpecId::FRONTIER" [] =
+    φ FRONTIER.
+  Proof. now intros; subst. Qed.
+  Smpl Add simple apply of_value_with_FRONTIER : of_value.
+
+  Lemma of_value_with_FRONTIER_THAWING :
+    Value.StructTuple "revm_primitives::hardfork::SpecId::FRONTIER_THAWING" [] =
+    φ FRONTIER_THAWING.
+  Proof. now intros; subst. Qed.
+  Smpl Add simple apply of_value_with_FRONTIER_THAWING : of_value.
+
+  Lemma of_value_with_HOMESTEAD :
+    Value.StructTuple "revm_primitives::hardfork::SpecId::HOMESTEAD" [] =
+    φ HOMESTEAD.
+  Proof. now intros; subst. Qed.
+  Smpl Add simple apply of_value_with_HOMESTEAD : of_value.
+
+  Lemma of_value_with_DAO_FORK :
+    Value.StructTuple "revm_primitives::hardfork::SpecId::DAO_FORK" [] =
+    φ DAO_FORK.
+  Proof. now intros; subst. Qed.
+  Smpl Add simple apply of_value_with_DAO_FORK : of_value.
+
+  Lemma of_value_with_TANGERINE :
+    Value.StructTuple "revm_primitives::hardfork::SpecId::TANGERINE" [] =
+    φ TANGERINE.
+  Proof. now intros; subst. Qed.
+  Smpl Add simple apply of_value_with_TANGERINE : of_value.
+
+  Lemma of_value_with_SPURIOUS_DRAGON :
+    Value.StructTuple "revm_primitives::hardfork::SpecId::SPURIOUS_DRAGON" [] =
+    φ SPURIOUS_DRAGON.
+  Proof. now intros; subst. Qed.
+  Smpl Add simple apply of_value_with_SPURIOUS_DRAGON : of_value.
+
+  Lemma of_value_with_BYZANTIUM :
+    Value.StructTuple "revm_primitives::hardfork::SpecId::BYZANTIUM" [] =
+    φ BYZANTIUM.
+  Proof. now intros; subst. Qed.
+  Smpl Add simple apply of_value_with_BYZANTIUM : of_value.
+
+  Lemma of_value_with_CONSTANTINOPLE :
+    Value.StructTuple "revm_primitives::hardfork::SpecId::CONSTANTINOPLE" [] =
+    φ CONSTANTINOPLE.
+  Proof. now intros; subst. Qed.
+  Smpl Add simple apply of_value_with_CONSTANTINOPLE : of_value.
+
+  Lemma of_value_with_PETERSBURG :
+    Value.StructTuple "revm_primitives::hardfork::SpecId::PETERSBURG" [] =
+    φ PETERSBURG.
+  Proof. now intros; subst. Qed.
+  Smpl Add simple apply of_value_with_PETERSBURG : of_value.
+
+  Lemma of_value_with_ISTANBUL :
+    Value.StructTuple "revm_primitives::hardfork::SpecId::ISTANBUL" [] =
+    φ ISTANBUL.
+  Proof. now intros; subst. Qed.
+  Smpl Add simple apply of_value_with_ISTANBUL : of_value.
+
+  Lemma of_value_with_MUIR_GLACIER :
+    Value.StructTuple "revm_primitives::hardfork::SpecId::MUIR_GLACIER" [] =
+    φ MUIR_GLACIER.
+  Proof. now intros; subst. Qed.
+  Smpl Add simple apply of_value_with_MUIR_GLACIER : of_value.
+
+  Lemma of_value_with_BERLIN :
+    Value.StructTuple "revm_primitives::hardfork::SpecId::BERLIN" [] =
+    φ BERLIN.
+  Proof. now intros; subst. Qed.
+  Smpl Add simple apply of_value_with_BERLIN : of_value.
+
+  Lemma of_value_with_LONDON :
+    Value.StructTuple "revm_primitives::hardfork::SpecId::LONDON" [] =
+    φ LONDON.
+  Proof. now intros; subst. Qed.
+  Smpl Add simple apply of_value_with_LONDON : of_value.
+
+  Lemma of_value_with_ARROW_GLACIER :
+    Value.StructTuple "revm_primitives::hardfork::SpecId::ARROW_GLACIER" [] =
+    φ ARROW_GLACIER.
+  Proof. now intros; subst. Qed.
+  Smpl Add simple apply of_value_with_ARROW_GLACIER : of_value.
+
+  Lemma of_value_with_GRAY_GLACIER :
+    Value.StructTuple "revm_primitives::hardfork::SpecId::GRAY_GLACIER" [] =
+    φ GRAY_GLACIER.
+  Proof. now intros; subst. Qed.
+  Smpl Add simple apply of_value_with_GRAY_GLACIER : of_value.
+
+  Lemma of_value_with_MERGE :
+    Value.StructTuple "revm_primitives::hardfork::SpecId::MERGE" [] =
+    φ MERGE.
+  Proof. now intros; subst. Qed.
+  Smpl Add simple apply of_value_with_MERGE : of_value.
+
+  Lemma of_value_with_SHANGHAI :
+    Value.StructTuple "revm_primitives::hardfork::SpecId::SHANGHAI" [] =
+    φ SHANGHAI.
+  Proof. now intros; subst. Qed.
+  Smpl Add simple apply of_value_with_SHANGHAI : of_value.
+
+  Lemma of_value_with_CANCUN :
+    Value.StructTuple "revm_primitives::hardfork::SpecId::CANCUN" [] =
+    φ CANCUN.
+  Proof. now intros; subst. Qed.
+  Smpl Add simple apply of_value_with_CANCUN : of_value.
+
+  Lemma of_value_with_PRAGUE :
+    Value.StructTuple "revm_primitives::hardfork::SpecId::PRAGUE" [] =
+    φ PRAGUE.
+  Proof. now intros; subst. Qed.
+  Smpl Add simple apply of_value_with_PRAGUE : of_value.
+
+  Lemma of_value_with_OSAKA :
+    Value.StructTuple "revm_primitives::hardfork::SpecId::OSAKA" [] =
+    φ OSAKA.
+  Proof. now intros; subst. Qed.
+  Smpl Add simple apply of_value_with_OSAKA : of_value.
+
+  Lemma of_value_with_AMSTERDAM :
+    Value.StructTuple "revm_primitives::hardfork::SpecId::AMSTERDAM" [] =
+    φ AMSTERDAM.
+  Proof. now intros; subst. Qed.
+  Smpl Add simple apply of_value_with_AMSTERDAM : of_value.
+
+  Definition of_value_FRONTIER :
+    OfValue.t (
+      Value.StructTuple "revm_primitives::hardfork::SpecId::FRONTIER" []
+    ).
+  Proof. econstructor; apply of_value_with_FRONTIER; eassumption. Defined.
+  Smpl Add simple apply of_value_FRONTIER : of_value.
+
+  Definition of_value_FRONTIER_THAWING :
+    OfValue.t (
+      Value.StructTuple "revm_primitives::hardfork::SpecId::FRONTIER_THAWING" []
+    ).
+  Proof. econstructor; apply of_value_with_FRONTIER_THAWING; eassumption. Defined.
+  Smpl Add simple apply of_value_FRONTIER_THAWING : of_value.
+
+  Definition of_value_HOMESTEAD :
+    OfValue.t (
+      Value.StructTuple "revm_primitives::hardfork::SpecId::HOMESTEAD" []
+    ).
+  Proof. econstructor; apply of_value_with_HOMESTEAD; eassumption. Defined.
+  Smpl Add simple apply of_value_HOMESTEAD : of_value.
+
+  Definition of_value_DAO_FORK :
+    OfValue.t (
+      Value.StructTuple "revm_primitives::hardfork::SpecId::DAO_FORK" []
+    ).
+  Proof. econstructor; apply of_value_with_DAO_FORK; eassumption. Defined.
+  Smpl Add simple apply of_value_DAO_FORK : of_value.
+
+  Definition of_value_TANGERINE :
+    OfValue.t (
+      Value.StructTuple "revm_primitives::hardfork::SpecId::TANGERINE" []
+    ).
+  Proof. econstructor; apply of_value_with_TANGERINE; eassumption. Defined.
+  Smpl Add simple apply of_value_TANGERINE : of_value.
+
+  Definition of_value_SPURIOUS_DRAGON :
+    OfValue.t (
+      Value.StructTuple "revm_primitives::hardfork::SpecId::SPURIOUS_DRAGON" []
+    ).
+  Proof. econstructor; apply of_value_with_SPURIOUS_DRAGON; eassumption. Defined.
+  Smpl Add simple apply of_value_SPURIOUS_DRAGON : of_value.
+
+  Definition of_value_BYZANTIUM :
+    OfValue.t (
+      Value.StructTuple "revm_primitives::hardfork::SpecId::BYZANTIUM" []
+    ).
+  Proof. econstructor; apply of_value_with_BYZANTIUM; eassumption. Defined.
+  Smpl Add simple apply of_value_BYZANTIUM : of_value.
+
+  Definition of_value_CONSTANTINOPLE :
+    OfValue.t (
+      Value.StructTuple "revm_primitives::hardfork::SpecId::CONSTANTINOPLE" []
+    ).
+  Proof. econstructor; apply of_value_with_CONSTANTINOPLE; eassumption. Defined.
+  Smpl Add simple apply of_value_CONSTANTINOPLE : of_value.
+
+  Definition of_value_PETERSBURG :
+    OfValue.t (
+      Value.StructTuple "revm_primitives::hardfork::SpecId::PETERSBURG" []
+    ).
+  Proof. econstructor; apply of_value_with_PETERSBURG; eassumption. Defined.
+  Smpl Add simple apply of_value_PETERSBURG : of_value.
+
+  Definition of_value_ISTANBUL :
+    OfValue.t (
+      Value.StructTuple "revm_primitives::hardfork::SpecId::ISTANBUL" []
+    ).
+  Proof. econstructor; apply of_value_with_ISTANBUL; eassumption. Defined.
+  Smpl Add simple apply of_value_ISTANBUL : of_value.
+
+  Definition of_value_MUIR_GLACIER :
+    OfValue.t (
+      Value.StructTuple "revm_primitives::hardfork::SpecId::MUIR_GLACIER" []
+    ).
+  Proof. econstructor; apply of_value_with_MUIR_GLACIER; eassumption. Defined.
+  Smpl Add simple apply of_value_MUIR_GLACIER : of_value.
+
+  Definition of_value_BERLIN :
+    OfValue.t (
+      Value.StructTuple "revm_primitives::hardfork::SpecId::BERLIN" []
+    ).
+  Proof. econstructor; apply of_value_with_BERLIN; eassumption. Defined.
+  Smpl Add simple apply of_value_BERLIN : of_value.
+
+  Definition of_value_LONDON :
+    OfValue.t (
+      Value.StructTuple "revm_primitives::hardfork::SpecId::LONDON" []
+    ).
+  Proof. econstructor; apply of_value_with_LONDON; eassumption. Defined.
+  Smpl Add simple apply of_value_LONDON : of_value.
+
+  Definition of_value_ARROW_GLACIER :
+    OfValue.t (
+      Value.StructTuple "revm_primitives::hardfork::SpecId::ARROW_GLACIER" []
+    ).
+  Proof. econstructor; apply of_value_with_ARROW_GLACIER; eassumption. Defined.
+  Smpl Add simple apply of_value_ARROW_GLACIER : of_value.
+
+  Definition of_value_GRAY_GLACIER :
+    OfValue.t (
+      Value.StructTuple "revm_primitives::hardfork::SpecId::GRAY_GLACIER" []
+    ).
+  Proof. econstructor; apply of_value_with_GRAY_GLACIER; eassumption. Defined.
+  Smpl Add simple apply of_value_GRAY_GLACIER : of_value.
+
+  Definition of_value_MERGE :
+    OfValue.t (
+      Value.StructTuple "revm_primitives::hardfork::SpecId::MERGE" []
+    ).
+  Proof. econstructor; apply of_value_with_MERGE; eassumption. Defined.
+  Smpl Add simple apply of_value_MERGE : of_value.
+
+  Definition of_value_SHANGHAI :
+    OfValue.t (
+      Value.StructTuple "revm_primitives::hardfork::SpecId::SHANGHAI" []
+    ).
+  Proof. econstructor; apply of_value_with_SHANGHAI; eassumption. Defined.
+  Smpl Add simple apply of_value_SHANGHAI : of_value.
+
+  Definition of_value_CANCUN :
+    OfValue.t (
+      Value.StructTuple "revm_primitives::hardfork::SpecId::CANCUN" []
+    ).
+  Proof. econstructor; apply of_value_with_CANCUN; eassumption. Defined.
+  Smpl Add simple apply of_value_CANCUN : of_value.
+
+  Definition of_value_PRAGUE :
+    OfValue.t (
+      Value.StructTuple "revm_primitives::hardfork::SpecId::PRAGUE" []
+    ).
+  Proof. econstructor; apply of_value_with_PRAGUE; eassumption. Defined.
+  Smpl Add simple apply of_value_PRAGUE : of_value.
+
+  Definition of_value_OSAKA :
+    OfValue.t (
+      Value.StructTuple "revm_primitives::hardfork::SpecId::OSAKA" []
+    ).
+  Proof. econstructor; apply of_value_with_OSAKA; eassumption. Defined.
+  Smpl Add simple apply of_value_OSAKA : of_value.
+
+  Definition of_value_AMSTERDAM :
+    OfValue.t (
+      Value.StructTuple "revm_primitives::hardfork::SpecId::AMSTERDAM" []
+    ).
+  Proof. econstructor; apply of_value_with_AMSTERDAM; eassumption. Defined.
+  Smpl Add simple apply of_value_AMSTERDAM : of_value.
+
+  Module SubPointer.
+
+  End SubPointer.
+End SpecId.
